while* -> loops
git-svn-id: https://www.lri.fr/svn/demons/why2/trunk@198 ecafba89-7d34-45a1-8a0b-92829e960b72

bench/good/loops_why.v
@@ -2,13 +2,123 @@
 Require Why.
 Require Omega.
 
+Lemma loop1_po_1 : 
+  (i: Z)
+  (Pre6: `i <= 10`)
+  (well_founded ? (Zwf ZERO)).
+Proof.
+Auto with datatypes.
+Save.
+
+Lemma loop1_po_2 : 
+  (i: Z)
+  (Pre6: `i <= 10`)
+  (Variant1: Z)
+  (i0: Z)
+  (Pre5: Variant1 = `10 - i0`)
+  (Pre4: `i0 <= 10`)
+  (Test2: `i0 < 10`)
+  (Pre3: `i0 <= 10`)
+  (i1: Z)
+  (Post1: i1 = `i0 + 1`)
+  `i1 <= 10` /\ (Zwf `0` `10 - i1` `10 - i0`).
+Proof.
+Unfold Zwf; Intros; Omega.
+Save.
+
+Lemma loop1_po_3 : 
+  (i: Z)
+  (Pre6: `i <= 10`)
+  (Variant1: Z)
+  (i0: Z)
+  (Pre5: Variant1 = `10 - i0`)
+  (Pre4: `i0 <= 10`)
+  (Test2: `i0 < 10`)
+  (Pre3: `i0 <= 10`)
+  (i1: Z)
+  (Post3: `i1 <= 10` /\ (Zwf `0` `10 - i1` `10 - i0`))
+  (Zwf `0` `10 - i1` Variant1).
+Proof.
+Intros. Rewrite Pre5; Tauto.
+Save.
+
+Lemma loop1_po_4 : 
+  (i: Z)
+  (Pre6: `i <= 10`)
+  (Variant1: Z)
+  (i0: Z)
+  (Pre5: Variant1 = `10 - i0`)
+  (Pre4: `i0 <= 10`)
+  (Test2: `i0 < 10`)
+  (Pre3: `i0 <= 10`)
+  (i1: Z)
+  (Post3: `i1 <= 10` /\ (Zwf `0` `10 - i1` `10 - i0`))
+  `i1 <= 10`.
+Proof.
+Intros. Simpl in Test2; Omega.
+Save.
+
+Lemma loop1_po_5 : 
+  (i: Z)
+  (Pre6: `i <= 10`)
+  (Variant1: Z)
+  (i0: Z)
+  (Pre5: Variant1 = `10 - i0`)
+  (Pre4: `i0 <= 10`)
+  (Test1: `i0 >= 10`)
+  (Pre2: `i0 <= 10`)
+  i0 = `10`.
+Proof.
+Simpl; Intros; Omega.
+Save.
+
+Definition loop1 := (* validation *)
+  [i: Z; Pre6: `i <= 10`]
+    (well_founded_induction Z (Zwf ZERO) (loop1_po_1 i Pre6) [Variant1: Z]
+      (i0: Z)(_: Variant1 = `10 - i0`)(_: `i0 <= 10`)
+      (sig_2 Z unit [i1:Z][result:unit](i1 = `10`))
+      [Variant1: Z; wf1: (Variant2: Z)(Pre1: (Zwf `0` Variant2 Variant1))
+       (i0: Z)(_: Variant2 = `10 - i0`)(_: `i0 <= 10`)
+       (sig_2 Z unit [i1:Z][result:unit](i1 = `10`)); i0: Z;
+       Pre5: Variant1 = `10 - i0`; Pre4: `i0 <= 10`]
+        let (result, Bool1) =
+          let (result1, Post4) = (Z_lt_ge_bool i0 `10`) in
+          (exist_1 [result2: bool]
+          (if result2 then `i0 < 10` else `i0 >= 10`) result1 Post4) in
+        (Cases (btest [result:bool](if result then `i0 < 10` else `i0 >= 10`)
+                result Bool1) of
+        | (left Test2) =>
+            let Pre3 = Pre4 in
+            let (i1, result0, Post6) =
+              let (i1, result0, Post3) =
+                let (i1, result0, Post1) =
+                  let (result0, Post1) = (exist_1 [result0: Z]
+                    result0 = `i0 + 1` `i0 + 1` (refl_equal ? `i0 + 1`)) in
+                  (exist_2 [i2: Z][result1: unit]i2 = `i0 + 1` result0 
+                  tt Post1) in
+                (exist_2 [i2: Z][result1: unit]`i2 <= 10` /\
+                (Zwf `0` `10 - i2` `10 - i0`) i1 result0
+                (loop1_po_2 i Pre6 Variant1 i0 Pre5 Pre4 Test2 Pre3 i1 Post1)) in
+              ((wf1 `10 - i1`)
+                (loop1_po_3 i Pre6 Variant1 i0 Pre5 Pre4 Test2 Pre3 i1 Post3)
+                i1 (refl_equal ? `10 - i1`)
+                (loop1_po_4 i Pre6 Variant1 i0 Pre5 Pre4 Test2 Pre3 i1 Post3)) in
+            (exist_2 [i2: Z][result1: unit]i2 = `10` i1 result0 Post6)
+        | (right Test1) =>
+            let Pre2 = Pre4 in
+            let (i1, result0, Post5) = (exist_2 [i1: Z][result0: unit]
+              i1 = `10` i0 tt
+              (loop1_po_5 i Pre6 Variant1 i0 Pre5 Pre4 Test1 Pre2)) in
+            (exist_2 [i2: Z][result1: unit]i2 = `10` i1 result0 Post5) end)
+      `10 - i` i (refl_equal ? `10 - i`) Pre6).
+
 Definition oppose := (* validation *)
   [u: unit; x: Z]
     let (result, Post1) = (exist_1 [result: Z]result = `(-x)` `(-x)`
       (refl_equal ? `(-x)`)) in
     (exist_2 [x1: Z][result0: unit]x1 = `(-x)` result tt Post1).
 
-Lemma test_po_1 : 
+Lemma loop2_po_1 : 
   (x: Z)
   (Pre4: `x <= 10`)
   (well_founded ? (Zwf ZERO)).
@@ -16,7 +126,7 @@ Proof.
 Auto with datatypes.
 Save.
 
-Lemma test_po_2 : 
+Lemma loop2_po_2 : 
   (x: Z)
   (Pre4: `x <= 10`)
   (Variant1: Z)
@@ -31,7 +141,7 @@ Proof.
 Unfold Zwf; Intros; Omega.
 Save.
 
-Lemma test_po_3 : 
+Lemma loop2_po_3 : 
   (x: Z)
   (Pre4: `x <= 10`)
   (Variant1: Z)
@@ -46,7 +156,7 @@ Proof.
 Intros; Rewrite Pre3; Tauto.
 Save.
 
-Lemma test_po_4 : 
+Lemma loop2_po_4 : 
   (x: Z)
   (Pre4: `x <= 10`)
   (Variant1: Z)
@@ -61,7 +171,7 @@ Proof.
 Intros; Intuition.
 Save.
 
-Lemma test_po_5 : 
+Lemma loop2_po_5 : 
   (x: Z)
   (Pre4: `x <= 10`)
   (Variant1: Z)
@@ -74,7 +184,7 @@ Proof.
 Simpl; Intros; Omega.
 Save.
 
-Lemma test_po_6 : 
+Lemma loop2_po_6 : 
   (x: Z)
   (Pre4: `x <= 10`)
   (x0: Z)
@@ -87,7 +197,7 @@ Proof.
 Intros; Omega.
 Save.
 
-Lemma test_po_7 : 
+Lemma loop2_po_7 : 
   (x: Z)
   (Pre4: `x <= 10`)
   (x0: Z)
@@ -98,10 +208,12 @@ Proof.
 Intros; Omega.
 Save.
 
-Definition test := (* validation *)
+
+
+Definition loop2 := (* validation *)
   [x: Z; Pre4: `x <= 10`]
     let (x0, result, Post5) =
-      (well_founded_induction Z (Zwf ZERO) (test_po_1 x Pre4) [Variant1: Z]
+      (well_founded_induction Z (Zwf ZERO) (loop2_po_1 x Pre4) [Variant1: Z]
         (x0: Z)(_: Variant1 = `10 - x0`)(_: `x0 <= 10`)
         (sig_2 Z unit [x1:Z][result:unit](x1 = `10`))
         [Variant1: Z; wf1: (Variant2: Z)(Pre1: (Zwf `0` Variant2 Variant1))
@@ -125,16 +237,16 @@ Definition test := (* validation *)
                     tt Post1) in
                   (exist_2 [x2: Z][result1: unit]`x2 <= 10` /\
                   (Zwf `0` `10 - x2` `10 - x0`) x1 result0
-                  (test_po_2 x Pre4 Variant1 x0 Pre3 Pre2 Test2 x1 Post1)) in
+                  (loop2_po_2 x Pre4 Variant1 x0 Pre3 Pre2 Test2 x1 Post1)) in
                 ((wf1 `10 - x1`)
-                  (test_po_3 x Pre4 Variant1 x0 Pre3 Pre2 Test2 x1 Post4) 
+                  (loop2_po_3 x Pre4 Variant1 x0 Pre3 Pre2 Test2 x1 Post4) 
                   x1 (refl_equal ? `10 - x1`)
-                  (test_po_4 x Pre4 Variant1 x0 Pre3 Pre2 Test2 x1 Post4)) in
+                  (loop2_po_4 x Pre4 Variant1 x0 Pre3 Pre2 Test2 x1 Post4)) in
               (exist_2 [x2: Z][result1: unit]x2 = `10` x1 result0 Post8)
           | (right Test1) =>
               let (x1, result0, Post7) = (exist_2 [x1: Z][result0: unit]
                 x1 = `10` x0 tt
-                (test_po_5 x Pre4 Variant1 x0 Pre3 Pre2 Test1)) in
+                (loop2_po_5 x Pre4 Variant1 x0 Pre3 Pre2 Test1)) in
               (exist_2 [x2: Z][result1: unit]x2 = `10` x1 result0 Post7) end)
         `10 - x` x (refl_equal ? `10 - x`) Pre4) in
     let (x1, result0, Post9) =
@@ -149,10 +261,10 @@ Definition test := (* validation *)
             let (x1, result3, Post13) = (oppose tt x0) in
             (exist_2 [x2: Z][result4: unit]x2 = `(-x0)` x1 result3 Post13) in
           (exist_2 [x2: Z][result2: unit]x2 = `(-10)` x1 result1
-          (test_po_6 x Pre4 x0 Post5 Test4 x1 Post12))
+          (loop2_po_6 x Pre4 x0 Post5 Test4 x1 Post12))
       | (right Test3) =>
           let (result1, Post11) = (exist_1 [result1: unit]x0 = `(-10)` 
-            tt (test_po_7 x Pre4 x0 Post5 Test3)) in
+            tt (loop2_po_7 x Pre4 x0 Post5 Test3)) in
           (exist_2 [x1: Z][result2: unit]x1 = `(-10)` x0 result1 Post11) end) in
     (Build_tuple_2 x1 result0).
 
